WIP

SystemF/More.lean
@@ -10,15 +10,9 @@ structure IsValCandidateRel (R : TmRel) : Prop where
   lc_left {t₁ t₂} : R t₁ t₂ → LcTm t₁
   lc_right {t₁ t₂} : R t₁ t₂ → LcTm t₂
 
-abbrev SemEnv := List TmRel
-
-/-- A dummy closed type for defining `ValRel` -/
-def Ty.dummy : Ty := .all (.bvar 0)
-
-theorem ty_dummy_lc : LcTy Ty.dummy := by
-  apply LcTy.all ∅
-  intros
-  constructor
+structure SemEnv where
+  bound : List TmRel
+  free  : Name → TmRel
 
 mutual
 
@@ -34,25 +28,26 @@ def ExpRel (T : Ty) (ρ : SemEnv) : TmRel :=
   if they are functions, applying the them yields related expressions -/
 def ValRel (T : Ty) (ρ : SemEnv) : TmRel :=
   match T with
-  | .bvar idx => if h : idx < ρ.length then ρ[idx] else fun _ _ => False
-  | .fvar name => fun _ _ => False
+  | .bvar idx => if h : idx < ρ.bound.length then ρ.bound[idx] else fun _ _ => False
+  | .fvar name => ρ.free name
   | .arr T₁ T₂ =>
     fun v₁ v₂ =>
       Value v₁ ∧ Value v₂ ∧ LcTm v₁ ∧ LcTm v₂ ∧
-      (∃ body₁, v₁ = (ƛ T₁ => body₁)) ∧
-      (∃ body₂, v₂ = (ƛ T₁ => body₂)) ∧
+      (∃ A₁ body₁, v₁ = (ƛ A₁ => body₁)) ∧
+      (∃ A₂ body₂, v₂ = (ƛ A₂ => body₂)) ∧
       ∀ arg₁ arg₂, ValRel T₁ ρ arg₁ arg₂ → ExpRel T₂ ρ (v₁ ◦ arg₁) (v₂ ◦ arg₂)
   | .all T =>
     fun v₁ v₂ =>
       Value v₁ ∧ Value v₂ ∧ LcTm v₁ ∧ LcTm v₂ ∧
       (∃ body₁, v₁ = (Λ' body₁)) ∧
       (∃ body₂, v₂ = (Λ' body₂)) ∧
-      ∀ R, IsValCandidateRel R → ExpRel T (R :: ρ) (v₁⦃Ty.dummy⦄) (v₂⦃Ty.dummy⦄)
+      ∀ R U₁ U₂, IsValCandidateRel R → LcTy U₁ →
+        LcTy U₂ → ExpRel T {ρ with bound := R :: ρ.bound} (v₁⦃U₁⦄) (v₂⦃U₂⦄)
 
 end
 
 def SemEnv.IsValid (ρ : SemEnv) : Prop :=
-  ∀ R ∈ ρ, IsValCandidateRel R
+  (∀ R ∈ ρ.bound, IsValCandidateRel R) ∧ (∀ X, IsValCandidateRel (ρ.free X))
 
 @[simp]
 theorem false_candidate : IsValCandidateRel (fun _ _ => False) := by
@@ -64,10 +59,14 @@ theorem valRel_candidate {T : Ty} {ρ : SemEnv} (hValid : ρ.IsValid) :
   induction T generalizing ρ with
   | bvar idx =>
     simp [ValRel]
-    by_cases h : idx < ρ.length
-    · aesop
+    by_cases h : idx < ρ.bound.length
+    · simp [SemEnv.IsValid] at hValid
+      aesop
     · simp [h]
-  | fvar name => simp [ValRel]
+  | fvar name =>
+    simp [ValRel]
+    simp [SemEnv.IsValid] at hValid
+    aesop
   | arr T₁ T₂ T₁_ih T₂_ih =>
     simp only [ValRel]
     constructor <;> aesop
@@ -123,7 +122,7 @@ lemma expRel_app {T₁ T₂ : Ty} {ρ : SemEnv} {t₁ t₂ u₁ u₂ : Tm}
   rcases ht with ⟨hLc_t₁, hLc_t₂, v_t₁, hEval₁, v_t₂, hEval_t₂, hVal⟩
   rcases hu with ⟨hLc_u₁, hLc_u₂, v_u₁, hEval_u₁, v_u₂, hEval_u₂, hVal_u⟩
   simp only [ValRel] at hVal
-  rcases hVal with ⟨hv_t₁, hv_t₂, hLc_vt₁, hLc_vt₂, ⟨body₁, rfl⟩, ⟨body₂, rfl⟩, f⟩
+  rcases hVal with ⟨hv_t₁, hv_t₂, hLc_vt₁, hLc_vt₂, ⟨A₁, body₁⟩, ⟨A₂, body₂⟩, f⟩
   have hExp_app := f v_u₁ v_u₂ hVal_u
   simp only [ExpRel, exists_and_left] at hExp_app
   rcases hExp_app with
@@ -148,21 +147,22 @@ lemma expRel_app {T₁ T₂ : Ty} {ρ : SemEnv} {t₁ t₂ u₁ u₂ : Tm}
             · exact hEval_final₂
         · exact hVal_final
 
-lemma expRel_lam {T₁ T₂ : Ty} {ρ : SemEnv} {t₁ t₂ : Tm}
-    (hLc_t₁ : LcTm (ƛ T₁ => t₁))
-    (hLc_t₂ : LcTm (ƛ T₁ => t₂))
+lemma expRel_lam {T₁ T₂ A₁ A₂ : Ty} {ρ : SemEnv} {t₁ t₂ : Tm}
+    (hLc_t₁ : LcTm (ƛ A₁ => t₁))
+    (hLc_t₂ : LcTm (ƛ A₂ => t₂))
     (hValid : ρ.IsValid)
     (hBody : ∀ v₁ v₂, ValRel T₁ ρ v₁ v₂ → ExpRel T₂ ρ (t₁⟪v₁⟫) (t₂⟪v₂⟫)) :
-    ExpRel (T₁ ⇒ T₂) ρ (ƛ T₁ => t₁) (ƛ T₁ => t₂) := by
+    ExpRel (T₁ ⇒ T₂) ρ (ƛ A₁ => t₁) (ƛ A₂ => t₂) := by
   simp only [ExpRel, exists_and_left]
   refine ⟨hLc_t₁, hLc_t₂, ?_⟩
-  use (ƛ T₁ => t₁)
+  use (ƛ A₁ => t₁)
   constructor
   · rfl
-  · use (ƛ T₁ => t₂)
+  · use (ƛ A₂ => t₂)
     constructor
     · rfl
-    · simp only [ValRel, Tm.lam.injEq, true_and, exists_eq']
+    · simp only [ValRel, Tm.lam.injEq, exists_and_left, ↓existsAndEq, and_true, exists_eq',
+      true_and]
       constructor
       · constructor
       · constructor
@@ -184,5 +184,316 @@ lemma expRel_lam {T₁ T₂ : Ty} {ρ : SemEnv} {t₁ t₂ : Tm}
                 · exact SmallStep.appLam _ _ _ hLc_t₂ hVal_arg₂
                 apply hBody
                 assumption
+
+lemma expRel_tLam {T : Ty} {ρ : SemEnv} {t₁ t₂ : Tm}
+    (hLc_t₁ : LcTm (Λ' t₁))
+    (hLc_t₂ : LcTm (Λ' t₂))
+    (hBody : ∀ R U₁ U₂, IsValCandidateRel R →
+      LcTy U₁ → LcTy U₂ →
+      ExpRel T { ρ with bound := R :: ρ.bound } ((Λ' t₁)⦃U₁⦄) ((Λ' t₂)⦃U₂⦄)) :
+    ExpRel (∀' T) ρ (Λ' t₁) (Λ' t₂) := by
+  simp only [ExpRel, exists_and_left]
+  refine ⟨hLc_t₁, hLc_t₂, ?_⟩
+  use (Λ' t₁)
+  constructor
+  · rfl
+  · use (Λ' t₂)
+    constructor
+    · rfl
+    · simp only [ValRel, Tm.tLam.injEq, exists_eq', true_and]
+      constructor
+      · constructor
+      · constructor
+        · constructor
+        · constructor
+          · assumption
+          · constructor
+            · assumption
+            · apply hBody
+
+lemma expRel_tApp {T T_arg U₁ U₂ : Ty} {ρ : SemEnv} {t₁ t₂ : Tm}
+    (hValid : ρ.IsValid)
+    (hLc_U₁ : LcTy U₁)
+    (hLc_U₂ : LcTy U₂)
+    (ht : ExpRel (∀' T) ρ t₁ t₂) :
+    ExpRel T { ρ with bound := ValRel T_arg ρ :: ρ.bound } (t₁⦃U₁⦄) (t₂⦃U₂⦄) := by
+  simp only [ExpRel, exists_and_left] at *
+  rcases ht with ⟨hLc_t₁, hLc_t₂, v₁, hEval₁, v₂, hEval₂, hVal⟩
+  simp only [ValRel] at hVal
+  rcases hVal with ⟨hv₁, hv₂, hLc_v₁, hLc_v₂, ⟨body₁, rfl⟩, ⟨body₂, rfl⟩, f⟩
+  have hExp_tApp := f (ValRel T_arg ρ) U₁ U₂ (valRel_candidate hValid) hLc_U₁ hLc_U₂
+  simp only [ExpRel, exists_and_left] at hExp_tApp
+  rcases hExp_tApp with
+    ⟨hLc_app₁, hLc_app₂, v_final₁, hEval_final₁, v_final₂, hEval_final₂, hVal_final⟩
+  constructor
+  · constructor <;> assumption
+  · constructor
+    · constructor <;> assumption
+    · use v_final₁
+      constructor
+      · apply Relation.ReflTransGen.trans
+        · exact multi_tApp hEval₁ hLc_U₁
+        · exact hEval_final₁
+      · use v_final₂
+        constructor
+        · apply Relation.ReflTransGen.trans
+          · exact multi_tApp hEval₂ hLc_U₂
+          · exact hEval_final₂
+        · exact hVal_final
+
+structure EnvRel (Γ : Context) (ρ : SemEnv) (δ₁ δ₂ : Name → Ty) (γ₁ γ₂ : Name → Tm) : Prop where
+  ty_rel {X} : (X, .ty) ∈ Γ →
+    IsValCandidateRel (ρ.free X) ∧ LcTy (δ₁ X) ∧ LcTy (δ₂ X)
+  tm_rel {x T} : (x, .tm T) ∈ Γ →
+    ValRel T ρ (γ₁ x) (γ₂ x)
+  δ₁_lc : ∀ X, LcTy (δ₁ X)
+  δ₂_lc : ∀ X, LcTy (δ₂ X)
+  γ₁_lc : ∀ x, LcTm (γ₁ x)
+  γ₂_lc : ∀ x, LcTm (γ₂ x)
+
+
+lemma expRel_eq_of_valRel_eq {ρ₁ ρ₂ : SemEnv} {T : Ty} (h : ValRel T ρ₁ = ValRel T ρ₂) :
+    ExpRel T ρ₁ = ExpRel T ρ₂ := by
+  funext t₁ t₂
+  simp [ExpRel]
+  simp [h]
+
+lemma valRel_free_update_of_not_mem {T : Ty} {X : Name} {ρ : SemEnv} {R : TmRel}
+    (hX : X ∉ T.fv) :
+    ValRel T { ρ with free := Function.update ρ.free X R } = ValRel T ρ := by
+  induction T generalizing ρ with
+  | bvar idx => simp [ValRel]
+  | fvar Y =>
+    have : Y ≠ X := by aesop
+    simp [ValRel, Function.update, this]
+  | arr T₁ T₂ T₁_ih T₂_ih =>
+    simp only [ValRel]
+    funext v₁ v₂
+    have hX₁ : X ∉ T₁.fv := by aesop
+    have hX₂ : X ∉ T₂.fv := by aesop
+    rw [T₁_ih hX₁]
+    have := @T₂_ih ρ hX₂
+    have := expRel_eq_of_valRel_eq this
+    rw [this]
+  | all T ih =>
+    simp only [ValRel]
+    funext v₁ v₂
+    have hX' : X ∉ T.fv := by aesop
+    have : ∀ R₁,
+        ExpRel T { bound := R₁ :: ρ.bound, free := Function.update ρ.free X R } =
+        ExpRel T { bound := R₁ :: ρ.bound, free := ρ.free } := by
+      intro R₁
+      let ρ' : SemEnv := { bound := R₁ :: ρ.bound, free := ρ.free }
+      have := ih (ρ := ρ') hX'
+      exact expRel_eq_of_valRel_eq this
+    simp [this]
+
+lemma expRel_openTy_comm {T : Ty} {X : Name} {ρ : SemEnv} {R : TmRel} {t₁ t₂ : Tm}
+    (hX : X ∉ T.fv) :
+    ExpRel T { ρ with bound := R :: ρ.bound } t₁ t₂ ↔
+    ExpRel (T⟪$TX⟫) { ρ with free := Function.update ρ.free X R } t₁ t₂ := by sorry
+
+/-- Opening a type syntactically is equivalent to evaluating that type into a `ValRel`
+  and pushing it onto the bound environment semantically. -/
+lemma expRel_openTy_bound_comm {T T_arg : Ty} {ρ : SemEnv} {t₁ t₂ : Tm} :
+    ExpRel T { ρ with bound := ValRel T_arg ρ :: ρ.bound } t₁ t₂ ↔
+    ExpRel (T⟪T_arg⟫) ρ t₁ t₂ := by
+  sorry
+
+
+theorem fundamental {Γ t T} (hTyp : Γ ⊢ t ∶ T)
+    {ρ δ₁ δ₂ γ₁ γ₂} (hValid : ρ.IsValid) (hEnv : EnvRel Γ ρ δ₁ δ₂ γ₁ γ₂) :
+    ExpRel T ρ (t.psubst γ₁ δ₁) (t.psubst γ₂ δ₂) := by
+  induction hTyp generalizing ρ δ₁ δ₂ γ₁ γ₂ with
+  | var Γ x T _ _ _ =>
+    simp only [Tm.psubst]
+    have := hEnv.tm_rel (by assumption)
+    exact expRel_of_valRel hValid this
+  | lam L Γ T₁ T₂ t _ h ih =>
+    simp only [Tm.psubst]
+    apply expRel_lam
+    · apply LcTm.lam (L ∪ t.fv)
+      · apply psubst_lcTy
+        · assumption
+        · exact hEnv.δ₁_lc
+      · intro x hX
+        rw [psubst_openTm_comm (by aesop) hEnv.γ₁_lc]
+        apply psubst_lcTm
+        · have := h x (by aesop) |> typing_regularity_tm
+          exact this
+        · intro y
+          by_cases hy : y = x
+          · simp [hy, Function.update]
+            constructor
+          · simp only [Function.update, hy, ↓reduceDIte]
+            exact hEnv.γ₁_lc y
+        · intro Y
+          exact hEnv.δ₁_lc Y
+    · apply LcTm.lam (L ∪ t.fv)
+      · apply psubst_lcTy
+        · assumption
+        · exact hEnv.δ₂_lc
+      · intro x hX
+        rw [psubst_openTm_comm (by aesop) hEnv.γ₂_lc]
+        apply psubst_lcTm
+        · have := h x (by aesop) |> typing_regularity_tm
+          exact this
+        · intro y
+          by_cases hy : y = x
+          · simp [hy, Function.update]
+            constructor
+          · simp only [Function.update, hy, ↓reduceDIte]
+            exact hEnv.γ₂_lc y
+        · intro Y
+          exact hEnv.δ₂_lc Y
+    · exact hValid
+    · intro v₁ v₂ hVal
+      have hLc_v₁ := valRel_candidate hValid |>.lc_left hVal
+      have hLc_v₂ := valRel_candidate hValid |>.lc_right hVal
+      have ⟨x, hx⟩ := exists_fresh_name (L ∪ t.fv)
+      let γ₁' := Function.update γ₁ x v₁
+      let γ₂' := Function.update γ₂ x v₂
+      have hEnv' : EnvRel ((x, .tm T₁) :: Γ) ρ δ₁ δ₂ γ₁' γ₂' := by
+        constructor
+        · intro X hX
+          have := hEnv.ty_rel (X := X) (by aesop)
+          aesop
+        · intro y T hy
+          by_cases hyx : y = x
+          · simp [hyx, γ₁', γ₂']
+            subst hyx
+            have hWf := h y (by aesop) |> typing_regularity_wf
+            have := wf_lookup_mid (Γ₁ := []) (b₂ := .tm T) hWf (by aesop)
+            aesop
+          · simp only [ne_eq, hyx, not_false_eq_true, Function.update_of_ne, γ₁', γ₂']
+            exact hEnv.tm_rel (by aesop)
+        · exact hEnv.δ₁_lc
+        · exact hEnv.δ₂_lc
+        · intro y
+          by_cases hyx : y = x
+          · simp only [hyx, Function.update_self, γ₁']
+            assumption
+          · simp only [ne_eq, hyx, not_false_eq_true, Function.update_of_ne, γ₁']
+            exact hEnv.γ₁_lc y
+        · intro y
+          by_cases hyx : y = x
+          · simp only [hyx, Function.update_self, γ₂']
+            assumption
+          · simp only [ne_eq, hyx, not_false_eq_true, Function.update_of_ne, γ₂']
+            exact hEnv.γ₂_lc y
+      have := ih x (by aesop) hValid hEnv'
+      rw [← psubst_openTm_comm', ← psubst_openTm_comm'] at this
+      · assumption
+      · aesop
+      · exact hEnv.γ₂_lc
+      · aesop
+      · exact hEnv.γ₁_lc
+  | app Γ t₁ t₂ T₁ T₂ _ _ ih₁ ih₂ =>
+    simp only [Tm.psubst]
+    apply expRel_app
+    · apply ih₁ hValid hEnv
+    · apply ih₂ hValid hEnv
+  | tLam L Γ t T h ih =>
+    simp only [Tm.psubst]
+    have hLc_v₁ : LcTm (Λ' Tm.psubst γ₁ δ₁ t) := by
+      apply LcTm.tLam (L ∪ t.fvTy)
+      intro X hX
+      rw [psubst_openTmTy_comm (by aesop) hEnv.γ₁_lc hEnv.δ₁_lc]
+      apply psubst_lcTm
+      · have := h X (by aesop) |> typing_regularity_tm
+        exact this
+      · exact hEnv.γ₁_lc
+      · intro Y
+        by_cases hY : Y = X
+        · simp [hY, Function.update]
+          constructor
+        · simp only [Function.update, hY, ↓reduceDIte]
+          exact hEnv.δ₁_lc Y
+    have hLc_v₂ : LcTm (Λ' Tm.psubst γ₂ δ₂ t) := by
+      apply LcTm.tLam (L ∪ t.fvTy)
+      intro X hX
+      rw [psubst_openTmTy_comm (by aesop) hEnv.γ₂_lc hEnv.δ₂_lc]
+      apply psubst_lcTm
+      · have := h X (by aesop) |> typing_regularity_tm
+        exact this
+      · exact hEnv.γ₂_lc
+      · intro Y
+        by_cases hY : Y = X
+        · simp [hY, Function.update]
+          constructor
+        · simp only [Function.update, hY, ↓reduceDIte]
+          exact hEnv.δ₂_lc Y
+    apply expRel_tLam
+    · assumption
+    · assumption
+    · intro R U₁ U₂ hR hLc_U₁ hLc_U₂
+      have ⟨X, hX⟩ := exists_fresh_name (L ∪ t.fvTy ∪ T.fv ∪ Context.fv Γ)
+      let δ₁' := Function.update δ₁ X U₁
+      let δ₂' := Function.update δ₂ X U₂
+      let ρ' := { ρ with bound := ρ.bound, free := Function.update ρ.free X R }
+      have hEnv' : EnvRel ((X, .ty) :: Γ) ρ' δ₁' δ₂' γ₁ γ₂ := by
+        constructor
+        · intro Y hY
+          by_cases hYX : Y = X
+          · simp [ρ', δ₁', δ₂', hYX, Function.update]
+            aesop
+          · simp [δ₁', δ₂', hYX]
+            have := hEnv.ty_rel (X := Y) (by aesop)
+            simp [ρ', hYX]
+            aesop
+        · intro x T' hx
+          have hx': (x, .tm T') ∈ Γ := by aesop
+          have := hEnv.tm_rel hx'
+          have : X ∉ T'.fv := by
+            have : X ∉ Context.fv Γ := by aesop
+            intro hIn
+            have : T'.fv ⊆ Context.fv Γ := subset_fv_of_mem_tm hx'
+            grind
+          have := valRel_free_update_of_not_mem (R := R) (ρ := ρ) this
+          simp only [this, ρ']
+          assumption
+        · intro Y
+          by_cases hY : Y = X
+          · simp only [hY, Function.update_self, δ₁']
+            assumption
+          · simp only [ne_eq, hY, not_false_eq_true, Function.update_of_ne, δ₁']
+            exact hEnv.δ₁_lc Y
+        · intro Y
+          by_cases hY : Y = X
+          · simp only [hY, Function.update_self, δ₂']
+            assumption
+          · simp only [ne_eq, hY, not_false_eq_true, Function.update_of_ne, δ₂']
+            exact hEnv.δ₂_lc Y
+        · exact hEnv.γ₁_lc
+        · exact hEnv.γ₂_lc
+      have hValid' : ρ'.IsValid := by
+        simp [SemEnv.IsValid] at hValid
+        simp only [SemEnv.IsValid]
+        simp only [ρ']
+        refine ⟨hValid.left, ?_⟩
+        intro Y
+        by_cases hY : Y = X
+        · simp only [Function.update, hY, ↓reduceDIte, eq_rec_constant]
+          exact hR
+        · simp only [Function.update, hY, ↓reduceDIte]
+          exact hValid.right Y
+      have := ih X (by aesop) hValid' hEnv'
+      apply expRel_step_back_right
+      · constructor <;> assumption
+      · apply SmallStep.tAppTLam <;> assumption
+      apply expRel_step_back_left
+      · constructor <;> assumption
+      · apply SmallStep.tAppTLam <;> assumption
+      rw [←expRel_openTy_comm (by aesop)] at this
+      rw [←psubst_openTmTy_comm' (by aesop) hEnv.γ₁_lc hEnv.δ₁_lc] at this
+      rw [←psubst_openTmTy_comm' (by aesop) hEnv.γ₂_lc hEnv.δ₂_lc] at this
+      assumption
+  | tApp Γ t T₁ T₂ _ _ ih =>
+    have hExp_t := ih hValid hEnv
+    have hLc_U₁ : LcTy (T₂.psubst δ₁) := sorry
+    have hLc_U₂ : LcTy (T₂.psubst δ₂) := sorry
+    have hApp := expRel_tApp (T_arg := T₂) hValid hLc_U₁ hLc_U₂ hExp_t
+    rw [expRel_openTy_bound_comm] at hApp
+    exact hApp
 
 end SystemF
